common/SmallstepClosed.v
@@ -1,0 +1,650 @@
+Require Import Relations.
+Require Import Wellfounded.
+Require Import Coqlib.
+Require Import Errors.
+Require Import Events.
+Require Import Globalenvs.
+Require Import LanguageInterface.
+Require Import Integers.
+Require Import Smallstep.
+Require Import Compiler.
+Import Values Maps Memory Ctypes AST.
+
+Set Implicit Arguments.
+
+Lemma E0_split : forall x y, E0 = x ** y -> x = E0 /\ y = E0.
+Proof.
+  unfold E0, Eapp. intros. split.
+  destruct x; auto. simpl in H. discriminate.
+  destruct y; auto. exfalso. apply (app_cons_not_nil _ _ _ H).
+Qed.
+
+Lemma open_bsim_simulation' {index state1 state2 liA1 liB1 liA2 liB2}:
+  forall
+    {L1 : lts liA1 liB1 state1} {L2 : lts liA2 liB2 state2}
+    {match_states: index -> state1 -> state2 -> Prop} {order},
+  (forall s2 t s2', Step L2 s2 t s2' ->
+   forall i s1, match_states i s1 s2 -> safe L1 s1 ->
+   exists i', exists s1',
+      (Plus L1 s1 t s1' \/ (Star L1 s1 t s1' /\ order i' i))
+   /\ match_states i' s1' s2') ->
+  forall s2 s2', Star L2 s2 E0 s2' ->
+  forall i s1, match_states i s1 s2 -> safe L1 s1 ->
+  exists i', exists s1', Star L1 s1 E0 s1'
+  /\ match_states i' s1' s2'.
+Proof.
+  intros until i. revert i. remember E0 as t. induction H0; simpl; intros.
+  exists i, s1. split; eauto. constructor.
+  subst t.
+  specialize (H _ _ _ H0 _ _ H3 H4) as (i'' & s & ST & MS).
+  apply E0_split in H2 as []. subst.
+  assert (Star L1 s0 E0 s). {
+    destruct ST.
+    inv H. apply E0_split in H6 as []. subst. eapply star_trans; eauto.
+    econstructor. exact H2.
+    econstructor. unfold E0, Eapp. rewrite app_nil_r. reflexivity.
+    tauto. tauto.
+  } clear ST.
+  eapply star_safe in H4; eauto.
+  specialize (IHstar ltac:(auto) _ _ MS H4) as (i' & s1' & ST & MS').
+  exists i', s1'. split; auto. eapply star_trans; eauto.
+Qed.
+
+Lemma open_progress' {index state1 state2 liA1 liB1 liA2 liB2}:
+  forall
+    {L1 : lts liA1 liB1 state1} {L2 : lts liA2 liB2 state2}
+    {match_states: index -> state1 -> state2 -> Prop} {order},
+  (forall i s1 s2,
+   match_states i s1 s2 -> safe L1 s1 ->
+   (exists r, final_state L2 s2 r) \/
+   (exists q, at_external L2 s2 q) \/
+   (exists t, exists s2', Step L2 s2 t s2')) ->
+  (forall s2 t s2', Step L2 s2 t s2' ->
+   forall i s1, match_states i s1 s2 -> safe L1 s1 ->
+   exists i', exists s1',
+      (Plus L1 s1 t s1' \/ (Star L1 s1 t s1' /\ order i' i))
+   /\ match_states i' s1' s2') ->
+  forall i s1 s2,
+  match_states i s1 s2 -> safe L1 s1 -> safe L2 s2.
+Proof.
+  intros. unfold safe. intros. revert i s1 H1 H2.
+  remember E0 as t.
+  induction H3; simpl; intros. eauto. subst t.
+  apply E0_split in H2 as []. subst.
+  exploit H0; eauto. intros (i' & s1' & ST & MS).
+  eapply IHstar. auto. exact MS.
+  assert (Star L1 s0 E0 s1'). {
+    destruct ST.
+    inv H2. apply E0_split in H8 as []. subst. eapply star_trans; eauto.
+    econstructor. exact H6.
+    econstructor. assert (E0 = E0 ** E0) by auto. exact H2. auto.
+    tauto.
+  } clear ST.
+  eapply star_safe; eauto.
+Qed.
+
+Module Closed.
+
+(* Definitions. *)
+
+Record semantics := ClosedSemantics_gen {
+  state: Type;
+  genvtype: Type;
+  step : genvtype -> state -> trace -> state -> Prop;
+  initial_state: state -> Prop;
+  final_state: state -> int -> Prop;
+  globalenv: genvtype;
+  symbolenv: Genv.symtbl
+}.
+
+Declare Scope closed_smallstep_scope.
+
+Notation " 'Step' L " := (step L (globalenv L)) (at level 1) : closed_smallstep_scope.
+Notation " 'Star' L " := (star (step L) (globalenv L)) (at level 1) : closed_smallstep_scope.
+Notation " 'Plus' L " := (plus (step L) (globalenv L)) (at level 1) : closed_smallstep_scope.
+Notation " 'Forever_silent' L " := (forever_silent (step L) (globalenv L)) (at level 1) : closed_smallstep_scope.
+Notation " 'Forever_reactive' L " := (forever_reactive (step L) (globalenv L)) (at level 1) : closed_smallstep_scope.
+Notation " 'Nostep' L " := (nostep (step L) (globalenv L)) (at level 1) : closed_smallstep_scope.
+Notation " 'Eventually' L " := (eventually (step L) (at_external L) (final_state L) (globalenv L)) (at level 1) : closed_smallstep_scope.
+Open Scope closed_smallstep_scope.
+
+
+Record fsim_properties (L1 L2: semantics) (index: Type)
+                       (order: index -> index -> Prop)
+                       (match_states: index -> state L1 -> state L2 -> Prop) : Prop := {
+    fsim_order_wf: well_founded order;
+    fsim_match_initial_states:
+      forall s1, initial_state L1 s1 ->
+      exists i, exists s2, initial_state L2 s2 /\ match_states i s1 s2;
+    fsim_match_final_states:
+      forall i s1 s2 r,
+      match_states i s1 s2 -> final_state L1 s1 r -> final_state L2 s2 r;
+    fsim_simulation:
+      forall s1 t s1', Step L1 s1 t s1' ->
+      forall i s2, match_states i s1 s2 ->
+      exists i', exists s2',
+         (Plus L2 s2 t s2' \/ (Star L2 s2 t s2' /\ order i' i))
+      /\ match_states i' s1' s2';
+    (* fsim_public_preserved:
+      forall id, Genv.public_symbol (symbolenv L2) id = Genv.public_symbol (symbolenv L1) id *)
+  }.
+
+Arguments fsim_properties: clear implicits.
+
+Inductive forward_simulation (L1 L2: semantics) : Prop :=
+  Forward_simulation (index: Type)
+                     (order: index -> index -> Prop)
+                     (match_states: index -> state L1 -> state L2 -> Prop)
+                     (props: fsim_properties L1 L2 index order match_states).
+
+Arguments Forward_simulation {L1 L2 index} order match_states props.
+
+
+Definition safe (L: semantics) (s: state L) : Prop :=
+  forall s',
+  Star L s E0 s' ->
+  (exists r, final_state L s' r)
+  \/ (exists t, exists s'', Step L s' t s'').
+
+Lemma star_safe:
+  forall (L: semantics) s s',
+  Star L s E0 s' -> safe L s -> safe L s'.
+Proof.
+  intros; red; intros. apply H0. eapply star_trans; eauto.
+Qed.
+
+Record bsim_properties (L1 L2: semantics) (index: Type)
+                       (order: index -> index -> Prop)
+                       (match_states: index -> state L1 -> state L2 -> Prop) : Prop := {
+    bsim_order_wf: well_founded order;
+    bsim_initial_states_exist:
+      forall s1, initial_state L1 s1 -> exists s2, initial_state L2 s2;
+    bsim_match_initial_states:
+      forall s1 s2, initial_state L1 s1 -> initial_state L2 s2 ->
+      exists i, exists s1', initial_state L1 s1' /\ match_states i s1' s2;
+    bsim_match_final_states:
+      forall i s1 s2 r,
+      match_states i s1 s2 -> safe L1 s1 -> final_state L2 s2 r ->
+      exists s1', Star L1 s1 E0 s1' /\ final_state L1 s1' r;
+    bsim_progress:
+      forall i s1 s2,
+      match_states i s1 s2 -> safe L1 s1 ->
+      (exists r, final_state L2 s2 r) \/
+      (exists t, exists s2', Step L2 s2 t s2');
+    bsim_simulation:
+      forall s2 t s2', Step L2 s2 t s2' ->
+      forall i s1, match_states i s1 s2 -> safe L1 s1 ->
+      exists i', exists s1',
+         (Plus L1 s1 t s1' \/ (Star L1 s1 t s1' /\ order i' i))
+      /\ match_states i' s1' s2';
+    (* bsim_public_preserved:
+      forall id, Genv.public_symbol (symbolenv L2) id = Genv.public_symbol (symbolenv L1) id *)
+  }.
+
+Arguments bsim_properties: clear implicits.
+
+Inductive backward_simulation (L1 L2: semantics) : Prop :=
+  Backward_simulation (index: Type)
+                      (order: index -> index -> Prop)
+                      (match_states: index -> state L1 -> state L2 -> Prop)
+                      (props: bsim_properties L1 L2 index order match_states).
+
+Arguments Backward_simulation {L1 L2 index} order match_states props.
+
+
+(* Closing open semantics. *)
+
+Section CLOSE_SEMANTICS.
+
+Variable liA liB : language_interface.
+Variable query : query liB.
+Variable reply : int -> reply liB -> Prop.
+Variable s : Smallstep.semantics liA liB.
+Variable se : Genv.symtbl.
+
+Definition close_semantics :=
+  let lts := Smallstep.activate s se in
+  {|
+    state := Smallstep.state s;
+    genvtype := Smallstep.genvtype lts;
+    step := Smallstep.step lts;
+    initial_state := Smallstep.initial_state lts query;
+    final_state := fun state retval => exists r, reply retval r /\ Smallstep.final_state lts state r;
+    globalenv := Smallstep.globalenv lts;
+    symbolenv := se;
+  |}.
+
+End CLOSE_SEMANTICS.
+
+Section CLOSE_SOUND.
+
+Variable liA1 liB1 : language_interface.
+Variable query1 : query liB1.
+Variable reply1 : int -> reply liB1 -> Prop.
+Variable s1 : Smallstep.semantics liA1 liB1.
+Variable se1 : Genv.symtbl.
+Definition lts1 := (Smallstep.activate s1 se1).
+Definition L1 := close_semantics query1 reply1 s1 se1.
+(* Hypothesis closed1 : forall s q, Smallstep.safe lts1 s -> ~ at_external lts1 s q. *)
+(* Hypothesis reply_sound1: forall r, exists i, reply1 i r. *)
+
+Variable liA2 liB2 : language_interface.
+Variable query2 : query liB2.
+Variable reply2 : int -> reply liB2 -> Prop.
+Variable s2 : Smallstep.semantics liA2 liB2.
+Variable se2 : Genv.symtbl.
+Definition lts2 := (Smallstep.activate s2 se2).
+Definition L2 := close_semantics query2 reply2 s2 se2.
+Hypothesis closed2 : forall s q, Smallstep.safe lts2 s -> ~ at_external lts2 s q.
+Hypothesis reply_sound2: forall s r, Smallstep.final_state lts2 s r -> exists i, reply2 i r.
+
+Variable ccA : callconv liA1 liA2.
+Variable ccB : callconv liB1 liB2.
+
+Hypothesis Hvalid : Genv.valid_for (skel s1) se1.
+
+Variable wB : ccworld ccB.
+
+Hypothesis Hmatch_query : match_query ccB wB query1 query2.
+Hypothesis Hmatch_reply : forall r r1 r2,
+  match_reply ccB wB r1 r2 ->
+  reply1 r r1 <-> reply2 r r2.
+
+Hypothesis Hmatch_senv : match_senv ccB wB se1 se2.
+
+Lemma close_sound_forward :
+  Smallstep.forward_simulation ccA ccB s1 s2 -> forward_simulation L1 L2.
+Proof.
+  (* pose proof (Hmatch_query := Hmatch_query).
+  pose proof (Hmatch_reply := Hmatch_reply).
+  pose proof (open_simulation := open_simulation).
+  pose proof (Hvalid := Hvalid). *)
+  intro open_simulation.
+  unfold Smallstep.forward_simulation in open_simulation.
+  inv open_simulation. inv X.
+  specialize (fsim_lts se1 se2 wB Hmatch_senv Hvalid). inv fsim_lts.
+  unfold L1, L2, close_semantics.
+  do 2 econstructor; simpl; eauto.
+
+  (* match final state *)
+  intros i s1' s2' r MS (r1 & R1 & FINAL).
+  exploit fsim_match_final_states0; eauto. intros (r2 & FINAL' & MATCH_REPLY).
+  eexists. split; eauto. eapply Hmatch_reply; eauto.
+Qed.
+
+Lemma safe_sound_1:
+  forall s, safe L1 s -> Smallstep.safe lts1 s.
+Proof.
+  unfold safe, Smallstep.safe, L1, lts1, close_semantics. simpl. intros.
+  specialize (H _ H0) as [(r & r0 & REPLY & FS)|(t & s'' & STEP)]; eauto.
+Qed.
+
+Lemma close_sound_backward:
+  Smallstep.backward_simulation ccA ccB s1 s2 -> backward_simulation L1 L2.
+Proof.
+  intro open_simulation.
+  unfold Smallstep.backward_simulation in open_simulation.
+  inv open_simulation. inv X.
+  specialize (bsim_lts se1 se2 wB Hmatch_senv Hvalid).
+  inv bsim_lts.
+  unfold L1, L2, close_semantics.
+  specialize (bsim_match_initial_states0 _ _ Hmatch_query).
+  inv bsim_match_initial_states0.
+  do 2 econstructor; simpl; simpl; eauto.
+
+  intros. specialize (bsim_match_cont_match _ _ H H0) as (s1' & IS & []).
+  exists x, s1'. eauto.
+
+  intros. apply safe_sound_1 in H0. destruct H1 as (r0 & REPLY & FS).
+  specialize (bsim_match_final_states0 _ _ _ _ H H0 FS) as (s1' & r1 & STAR & FS' & MS).
+  exists s1'. split; eauto. eexists. split; eauto. eapply Hmatch_reply; eauto.
+
+  intros. apply safe_sound_1 in H0.
+  pose proof (progress := bsim_progress0).
+  specialize (bsim_progress0 _ _ _ H H0) as [(r & FS)|[|]].
+  left. destruct (reply_sound2 _ _ FS) as (ri & REPLY). eauto.
+  destruct H1. exfalso. eapply closed2; eauto. eapply open_progress'; eauto.
+  auto.
+
+  intros. apply safe_sound_1 in H1.
+  eapply bsim_simulation0; eauto.
+Qed.
+
+End CLOSE_SOUND.
+
+Section CLOSE_COMPCERT.
+
+Variable p : Csyntax.program.
+Variable tp : Asm.program.
+Hypothesis transf : transf_c_program p = OK tp.
+Let se := Genv.symboltbl (erase_program p).
+
+Variable main_block_c : block.
+Variable m0_c : mem.
+
+Let liA1 := li_c.
+Let liB1 := li_c.
+Let sg := AST.mksignature nil (AST.Tret AST.Tint) AST.cc_default.
+Let main_function_value_c := Vptr main_block_c Ptrofs.zero.
+Let query1 := cq main_function_value_c sg nil m0_c.
+Inductive reply1 : int -> c_reply -> Prop :=
+  | reply1_intro: forall r m,
+      reply1 r (cr (Vint r) m).
+Let s1 := Csem.semantics p.
+Let se1 := se.
+Let lts1' := (Smallstep.activate s1 se1).
+
+Let ge_c' := Smallstep.globalenv (s1 se).
+Let ge_c := Csem.genv_genv ge_c'.
+Variable main_c : Csyntax.fundef.
+Hypothesis Hinitial_state_c :
+  Genv.init_mem (erase_program p) = Some m0_c /\
+  Genv.find_symbol se p.(prog_main) = Some main_block_c /\
+  Genv.find_funct_ptr ge_c main_block_c = Some main_c.
+
+Import Asm.
+
+Let s2 := Asm.semantics tp.
+Let ge_asm := Smallstep.globalenv (s2 se).
+Variable m0_asm : mem.
+Hypothesis Hinitial_state_asm :
+  Genv.init_mem (erase_program tp) = Some m0_asm.
+
+Let liA2 := li_asm.
+Let liB2 := li_asm.
+Let rs0 :=
+    (Pregmap.init Vundef)
+    # PC <- (Genv.symbol_address ge_asm tp.(prog_main) Ptrofs.zero)
+    # RA <- Vnullptr
+    # RSP <- Vnullptr.
+Let query2 := (rs0, m0_asm).
+Inductive reply2: int -> (regset * mem) -> Prop :=
+  | reply2_intro: forall r rs m,
+      rs#PC = Vnullptr ->
+      rs#RAX = Vint r ->
+      reply2 r (rs, m).
+Let se2 := se.
+Let lts2' := (Smallstep.activate s2 se2).
+
+Ltac clean_destr :=
+  match goal with
+  | H: _ = left _ |- _ => clear H
+  | H: _ = right _ |- _ => clear H
+  end.
+
+Ltac destr :=
+  match goal with
+    |- context [match ?a with _ => _ end] => destruct a eqn:?; try intuition congruence
+  end; repeat clean_destr.
+
+Ltac destr_in H :=
+  match type of H with
+    context [match ?a with _ => _ end] => destruct a eqn:?; try intuition congruence
+  | _ => inv H
+  end; repeat clean_destr.
+
+Lemma erase_same: erase_program p = erase_program tp.
+Proof.
+  exploit transf_c_program_match; eauto. intro MATCH.
+  unfold match_c_prog in MATCH. simpl in MATCH. repeat destruct MATCH as (? & MATCH).
+  fold Csyntax.fundef. remember p as xx.
+  rename xx into p', p into xx. rename p' into p.
+  match goal with
+  | H: ?P p ?p2 |- _ => rewrite Heqxx in H
+  end.
+  rewrite Heqxx. clear Heqxx.
+  Ltac mp H p1 p2 :=
+    unfold Linking.match_program in H;
+    match type of H with
+    | Linking.match_program_gen _ _ _ _ _ =>
+        apply Linking.match_program_skel in H;
+        try fold CminorSel.fundef in H;
+        try fold RTL.fundef in H;
+        rewrite H; clear H p1;
+        rename p2 into p1
+    | Linking.match_program_gen _ _ _ _ _ /\ _ =>
+        let H' := fresh "H" in
+        let garbage := fresh "H" in
+        destruct H as (H' & garbage);
+        clear garbage;
+        mp H' p1 p2
+    end.
+  Ltac try_rewrite xx := match goal with
+  | H: ?P xx ?p2 |- _ =>
+    unfold P in H; mp H xx p2
+  | H: match_if ?cond ?P xx ?p2 |- _ =>
+    unfold match_if, P in H;
+    let H' := fresh "H" in
+    assert (H' : erase_program xx = erase_program p2) by (destr_in H; mp H xx p2; auto);
+    rewrite H';
+    clear H' H xx;
+    rename p2 into xx
+  end.
+  repeat try_rewrite xx.
+  unfold Unusedglobproof.match_prog in H12.
+  destruct H12 as (u & VALID & MATCH').
+  inv MATCH'. rewrite <- match_prog_skel.
+  clear match_prog_main match_prog_public match_prog_def match_prog_skel VALID xx u.
+  rename x12 into xx.
+  repeat try_rewrite xx.
+  auto.
+Qed.
+
+Lemma m0_same: m0_c = m0_asm.
+Proof.
+  rewrite erase_same, Hinitial_state_asm in Hinitial_state_c.
+  destruct Hinitial_state_c. inv H. auto.
+Qed.
+
+Let ccA : callconv liA1 liA2 := cc_compcert.
+Let ccB : callconv liB1 liB2 := cc_compcert.
+
+Lemma Hvalid: Genv.valid_for (erase_program p) se1.
+Proof.
+  red. intros. rewrite Genv.find_info_symbol in H. destruct H as (b & []).
+  exists b, g. unfold se1, se. split; auto. split; auto.
+  destruct g; constructor. constructor.
+  destruct v. constructor; constructor.
+Qed.
+
+Lemma m0_inject: Mem.inject (Mem.flat_inj (Mem.support m0_c)) m0_c m0_asm.
+Proof.
+  rewrite <- m0_same.
+  apply (Genv.initmem_inject (erase_program p)).
+  destruct Hinitial_state_c. auto.
+Qed.
+
+Let wB : ccworld ccB.
+  unfold ccB, cc_compcert, CA.cc_c_asm_injp. simpl.
+  (* ro *)
+  split. split. exact se. split. exact se. exact m0_asm.
+  (* wt_c *)
+  split. split. exact se. split. exact se. exact sg.
+  (* cc_c_asm_injp *)
+  split. split. exact se. split.
+  simpl. econstructor. exact m0_inject. exact sg. exact rs0.
+  (* cc_asm injp *)
+  econstructor. exact m0_inject.
+Defined.
+
+Hypothesis closed:
+  forall v id sg, Genv.find_funct (Genv.globalenv se tp) v <> Some (External (EF_external id sg)).
+
+Lemma closed2 : forall s q, Smallstep.safe lts2' s -> ~ Smallstep.at_external lts2' s q.
+Proof.
+  unfold lts2', s2, se2, semantics. simpl. intros. intro.
+  destruct s. inv H0.
+  eapply closed; eauto.
+Qed.
+
+Lemma reply_sound2: forall s r, Smallstep.final_state lts2' s r -> exists i, reply2 i r.
+Proof.
+  unfold lts2', s2, se2. simpl. intros. destruct s.
+  inversion H.
+  give_up.
+Admitted.
+
+Lemma romem_for_symtbl_sound:
+  ValueAnalysis.romem_for_symtbl se = ValueAnalysis.romem_for p.
+Proof.
+  unfold ValueAnalysis.romem_for, ValueAnalysis.romem_for_symtbl. unfold se.
+  unfold Genv.symboltbl.
+  destruct Hinitial_state_c as (INIT & SYM & FPTR).
+Abort.
+
+Lemma sound_memory_ro: ValueAnalysis.sound_memory_ro se m0_c.
+Proof.
+  unfold se. destruct Hinitial_state_c. clear H0.
+  constructor.
+  apply ValueAnalysis.initial_mem_matches' in H as (? & ? & ? & ROM & ?).
+  2:intros; inv H0; auto.
+  specialize (ROM p ltac:(apply Linking.linkorder_refl)).
+  admit.
+  erewrite Genv.init_mem_genv_sup; eauto.
+Admitted.
+
+Lemma main_block_genv: Genv.find_symbol se (prog_main tp) = Some main_block_c.
+Proof.
+  destruct Hinitial_state_c as [? []].
+  pose proof erase_same. inv H2. simpl in H0. rewrite H0. auto.
+Qed.
+
+Lemma has_main_block: sup_In main_block_c (Mem.support m0_c).
+Proof.
+  destruct Hinitial_state_c as [? []].
+  eapply Genv.find_symbol_not_fresh; eauto.
+Qed.
+
+Lemma Hmatch_query : match_query ccB wB query1 query2.
+Proof.
+  simpl.
+  exists query1. split.
+  constructor. rewrite <- m0_same. constructor. exact sound_memory_ro.
+  exists query1. split.
+  constructor. split. reflexivity. simpl. auto.
+  exists query2. split.
+  unfold query1, query2. econstructor; simpl.
+  unfold Conventions1.loc_arguments. cbn.
+  destruct Archi.ptr64, Archi.win64; simpl; constructor.
+  unfold rs0. simpl.
+  unfold main_function_value_c, Genv.symbol_address.
+  rewrite main_block_genv.
+  econstructor. unfold Mem.flat_inj. pose proof has_main_block. destr.
+  rewrite Ptrofs.add_zero. auto.
+  intros. inv H.
+  cbn. unfold Vnullptr, Tptr. destruct Archi.ptr64; simpl; auto.
+  cbn. unfold Vnullptr, Tptr. destruct Archi.ptr64; simpl; auto.
+  give_up. (* rs0 RSP = Vnullptr *)
+  econstructor.
+  unfold Conventions.tailcall_possible, Conventions.size_arguments, Conventions1.loc_arguments. simpl.
+  destruct Archi.ptr64, Archi.win64; simpl; auto.
+  unfold main_function_value_c. discriminate.
+  discriminate.
+  unfold cc_asm_match'. simpl. split; [|split].
+  intros. unfold rs0.
+  destruct (PregEq.eq r RSP); [subst; rewrite Pregmap.gss|
+  rewrite Pregmap.gso; auto; destruct (PregEq.eq r RA); [subst; rewrite Pregmap.gss|
+  rewrite Pregmap.gso; auto; destruct (PregEq.eq r PC); [subst; rewrite Pregmap.gss|
+  rewrite Pregmap.gso; auto]]].
+  unfold Vnullptr. destr; constructor.
+  unfold Vnullptr. destr; constructor.
+  unfold Genv.symbol_address. destr; econstructor.
+  unfold ge_asm in Heqo. simpl in Heqo. rewrite main_block_genv in Heqo. inv Heqo.
+  unfold Mem.flat_inj. pose proof has_main_block. destr.
+  rewrite Ptrofs.add_zero. auto.
+  unfold rs0.
+  rewrite Pregmap.gso; [|discriminate].
+  rewrite Pregmap.gso; [|discriminate].
+  rewrite Pregmap.gss.
+  unfold ge_asm. simpl. unfold Genv.symbol_address. rewrite main_block_genv. discriminate.
+  rewrite <- m0_same at 2. constructor.
+Admitted.
+
+Lemma Hmatch_reply : forall r r1 r2,
+  match_reply ccB wB r1 r2 ->
+  reply1 r r1 <-> reply2 r r2.
+Proof.
+  simpl. intros.
+  destruct H, H, H0, H0, H1, H1.
+  split; intro r'; inv r'.
+
+  inv H. inv H0. inv H1. inv H2. destruct r2.
+  inv H0. simpl in H2. inv H2.
+  unfold rs0 in H16.
+  rewrite Pregmap.gso in H16; [|discriminate]. rewrite Pregmap.gss in H16.
+  assert (r0 PC = Vnullptr). {
+    pose proof (INJ := H0 PC). rewrite H16 in INJ.
+    unfold Vnullptr. unfold Vnullptr in INJ.
+    destruct Archi.ptr64; inv INJ; auto.
+  }
+  constructor; auto.
+  unfold Conventions1.loc_result, Conventions1.loc_result_64, Conventions1.loc_result_32 in tres.
+  subst tres.
+  destr_in H10; simpl in H10; inv H10;
+  specialize (H0 RAX); rewrite <- H7 in H0; inv H0; auto.
+
+  inv H2. inv H5. destruct x1. simpl in H6. inv H6.
+  specialize (H5 RAX). rewrite H4 in H5. inv H5.
+  inv H1. destruct r1.
+  inv H. destruct H1. inv H0. unfold sg, proj_sig_res in H5. simpl in H5.
+  assert (res = Vint r). {
+    unfold Conventions1.loc_result, Conventions1.loc_result_64, Conventions1.loc_result_32 in tres.
+    subst tres. destr_in H15; simpl in H15.
+    rewrite <- H8 in H15. inv H15. auto.
+    give_up. (* Vundef *)
+    rewrite <- H8 in H15. inv H15. auto.
+    give_up.
+  }
+  subst res. constructor.
+  inv H1. destruct r1.
+  inv H. inv H0.
+  unfold Conventions1.loc_result, Conventions1.loc_result_64, Conventions1.loc_result_32 in tres.
+  subst tres. destr_in H15; simpl in H15; rewrite <- H8 in H15; inv H15.
+  give_up.
+  give_up.
+Admitted.
+
+Lemma Hmatch_senv : match_senv ccB wB se1 se2.
+Proof.
+  unfold ccB, cc_compcert, se1, se2. simpl.
+  split; [|split; [|split]].
+
+  constructor. auto.
+  constructor. auto.
+
+  destruct Hinitial_state_c as (INIT & ? & ?).
+  unfold se. unfold Mem.flat_inj.
+  constructor.
+  split; try erewrite Genv.init_mem_genv_sup by eauto; auto; intros.
+  exists b1. destr.
+  exists b2. destr.
+  1,2,3:destr_in H1.
+  1,2:erewrite Genv.init_mem_genv_sup by eauto. 2:rewrite m0_same.
+  1,2:apply Mem.sup_include_refl.
+
+  destruct Hinitial_state_c as (INIT & ? & ?).
+  unfold se. unfold Mem.flat_inj.
+  constructor.
+  split; try erewrite Genv.init_mem_genv_sup by eauto; auto; intros.
+  exists b1. destr.
+  exists b2. destr.
+  1,2,3:destr_in H1.
+  1,2:erewrite Genv.init_mem_genv_sup by eauto. 2:rewrite m0_same.
+  1,2:apply Mem.sup_include_refl.
+Qed.
+
+Lemma open_simulation: Smallstep.backward_simulation ccA ccB s1 s2.
+Proof.
+  apply c_semantic_preservation, transf_c_program_match. auto.
+Qed.
+
+Lemma compcert_close_sound :
+  backward_simulation (L1 query1 reply1 s1 se1) (L2 query2 reply2 s2 se2).
+Proof.
+  eapply close_sound_backward; eauto using
+    closed2, reply_sound2, Hvalid, Hmatch_query, Hmatch_reply, Hmatch_senv, open_simulation.
+Qed.
+
+End CLOSE_COMPCERT.
+
+End Closed.
